OddOrder.lean
@@ -18,6 +18,7 @@ import OddOrder.GroupTheory.CriticalSubgroup
 import OddOrder.GroupTheory.ElementaryAbelian
 import OddOrder.GroupTheory.ElementaryAbelianFamily
 import OddOrder.GroupTheory.FrattiniPGroup
+import OddOrder.GroupTheory.HallCollection
 import OddOrder.GroupTheory.IsExtraspecial
 import OddOrder.GroupTheory.IsMetacyclic
 import OddOrder.GroupTheory.MackeyTransfer
